Working partial map version

natexp_compiler.v
@@ -13,48 +13,44 @@ Rocq aware of the fact that the compiled code will never lead to a run time erro
  *)
 
 Require Import Stdlib.Strings.String.
+Require Import Stdlib.Lists.List.
 
 (*
 Inductive definition:
  *)
 
 Definition lit := nat. 
+Definition binop := (lit -> lit -> lit). 
+
+(*Partial map*)
+(*
 Definition env := string -> option lit.
 Definition empty : env := (fun _ => None).
 Definition update (f : env) (x : string) (l : lit) : env :=
   (fun y => if String.eqb x y then Some l else f y).
+ *)
+
+(*Total map: Defaults to 0*)
+Definition env := string -> lit.
+Definition empty : env := (fun _ => 0).
+Definition update (f : env) (x : string) (l : lit) : env :=
+  (fun y => if String.eqb x y then l else f y).
+
 Inductive Exp : Set :=
   | Elit : lit -> Exp
   | Evar : string -> Exp
-  | Eplus : Exp -> Exp -> Exp
-  | Emin : Exp -> Exp -> Exp
-  | Emult : Exp -> Exp -> Exp.
-
-
+  | Ebinop : binop -> Exp -> Exp -> Exp
+.
 (*
 Semantics for Exp
  *)
-Fixpoint eval (e:Exp) (f:env) {struct e} : option lit :=
+Fixpoint eval (e:Exp) (f:env) {struct e} : lit :=
 match e with
-| Elit l      => Some l
+| Elit l      => l
 | Evar x      => f x
-| Eplus e1 e2 => 
-    match eval e1 f, eval e2 f with
-    | Some l1, Some l2 => Some (plus l1 l2)
-    | _,_ => None
-    end
-| Emin  e1 e2 =>
-    match eval e1 f, eval e2 f with
-    | Some l1, Some l2 => Some (min l1 l2)
-    | _,_ => None
-    end
-| Emult e1 e2 => 
-    match eval e1 f, eval e2 f with
-    | Some l1, Some l2 => Some (mult l1 l2)
-    | _,_ => None
-    end
+| Ebinop op e1 e2 => op (eval e1 f) (eval e2 f)
 end.
-
+(*
 Definition exp0 := Elit 0.
 Definition exp1 := Elit 1.
 Definition exp2 := Evar "x".
@@ -68,64 +64,93 @@ Eval compute in (eval exp3 empty).
 Eval compute in (eval exp3 env0).
 Eval compute in (eval exp3 env1).
 Eval compute in (eval exp3 env2).
-
+ *)
 
 (*
-   Inductive definition RPN
+Stackbased Implementation 
  *)
+ 
 Inductive RPN : Set :=
   | RPNlit : lit -> RPN
   | RPNvar : string -> RPN
-  | RPNbinop : option RPN -> option RPN -> (lit -> lit -> lit) -> RPN
+  | RPNbinop : binop -> RPN
 .
 
-(*
-   Compiler from Exp to RPN
- *)
-Fixpoint rpn (e:Exp) {struct e} : RPN :=
+
+Fixpoint rpn (e:Exp) {struct e} : list RPN :=
 match e with
-| Elit l => RPNlit l
-| Evar x => RPNvar x
-| Eplus e1 e2 => RPNbinop (Some (rpn e1)) (Some (rpn e2)) plus
-| Emin  e1 e2 => RPNbinop (Some (rpn e1)) (Some (rpn e2)) min
-| Emult e1 e2 => RPNbinop (Some (rpn e1)) (Some (rpn e2)) mult
+| Elit l => RPNlit l :: nil
+| Evar s => RPNvar s :: nil
+| Ebinop op e1 e2 => rpn e1 ++ rpn e2 ++ RPNbinop op :: nil
 end.
 
+Fixpoint rpn_eval (inp: list RPN) (stack: list lit) (f : env) {struct inp} : option lit :=
+match inp with
+| nil => 
+  match stack with
+  | x::xs => Some x
+  | nil  => None
+  end
+| (RPNlit   l ) :: rs => rpn_eval rs (l  ::stack) f
+| (RPNvar   s ) :: rs => rpn_eval rs (f s::stack) f
+| (RPNbinop op) :: rs =>
+  match stack with
+  | x::x'::xs => rpn_eval rs ((op x' x)::xs) f
+  | _         => None
+  end
+end.
+
+Definition rpn0:(list RPN) := (RPNlit 1) :: (RPNlit 2) :: (RPNbinop plus)::nil.
+Definition rpn1:(list RPN) := (RPNlit 3) :: (RPNlit 1) :: (RPNlit 2) :: (RPNbinop plus) :: (RPNbinop plus)::nil.
+Definition rpn2:(list RPN) := (RPNlit 3) :: (RPNlit 1) :: (RPNlit 2) :: (RPNbinop plus) :: (RPNbinop mult)::nil.
+Eval compute in (rpn_eval (rpn2) nil empty).
+Definition rpn3:(list RPN) := (RPNvar "x") :: (RPNlit 2) :: (RPNbinop plus)::nil.
 (*
-  Evaluator for RPN
+Eval compute in (rpn_eval (rpn3) nil env0).
+Eval compute in (rpn_eval (rpn3) nil empty).
  *)
 
-Fixpoint rpn_eval (r:RPN) (f:env) {struct r} : option lit :=
-match r with
-| RPNlit l => Some l
-| RPNvar x => f x
-| RPNbinop (Some r1) (Some r2) op => 
-    match (rpn_eval r1 f), (rpn_eval r2 f) with
-    | Some r1', Some r2' => Some (op r1' r2')
-    | _, _ => None
-    end
-| _ => None
-end.
+Lemma rpn_applied :
+  forall (e : Exp) (f : env) (st : list lit) (code : list RPN),
+    rpn_eval (rpn e ++ code) st f =
+    rpn_eval code (eval e f :: st) f.
+Proof.
+  (* We do not need to use a different environment in the induction step*)
+  intros e f.
+  (* Induction on the expressions*)
+  induction e;
+  (* Solve trivial cases (Lit and Var) *)
+  simpl; try reflexivity.
+  (* Solve Binop case*)
+  - intros st code.
+    (* Reshuffle list to get into a form of (rpn e1 ++ (rpn e2 ++ code)) *)
+    rewrite <- app_assoc. 
+    rewrite <- app_assoc. 
+    rewrite <- app_comm_cons. 
+    simpl. 
+    (* Rewrite the IHs *)
+    rewrite IHe1. 
+    rewrite IHe2. 
+    reflexivity.
+Qed.
 
-Definition rpn0 := RPNlit 0.
-Definition rpn1 := RPNbinop (Some (RPNlit 5)) (Some (RPNlit 6)).
-Definition rpn2 := RPNbinop (Some (RPNvar "x")) (Some (RPNlit 6)).
-Definition rpn3 := RPNbinop None (Some (RPNlit 6)).
-Eval compute in (rpn_eval (rpn1 plus) empty).
-Eval compute in (rpn_eval (rpn1 mult) empty).
-Eval compute in (rpn_eval (rpn2 plus) empty).
-Eval compute in (rpn_eval (rpn2 plus) env0 ).
-Eval compute in (rpn_eval (rpn2 plus) env1 ).
-Eval compute in (rpn_eval (rpn2 plus) env2 ).
 
 (*
 Prove that
 forall e:Exp, Some (eval e) = rpn_eval (rpn e)
  *)
-
-Lemma Equivalence_Eval_RPNEval : forall e:Exp, eval e = rpn_eval (rpn e).
+Lemma equivalent_under_extensionality : forall (f:env) (e:Exp), 
+  Some (eval e f) = rpn_eval (rpn e) nil f.
 Proof.
-  induction e; simpl; try rewrite <- IHe1, <- IHe2; reflexivity.
+  intros f e.
+  (* Delay the inductive step to the helper Lemma rpn_applied *)
+  destruct e; 
+  (* Solve trivial cases (Lit and Var) *)
+  simpl; try reflexivity.
+  (* Solve Binop case by applying the rpn_eval twice*)
+  - rewrite rpn_applied.
+    rewrite rpn_applied.
+    reflexivity.
 Qed.
 
 (*
@@ -136,40 +161,9 @@ ization in Rocq.
 
 ANSWER:
 We can make it a relation which should hold for all Exp. This means that
-we do not need to include None terms as we check for all possible expressions. 
-Now if we prove this relation we prove the equivalence.
+we do not need to include None terms as we check for all possible expressions,
+which can not be None when translated with rpn.
+
+Now if we prove this relation we prove the equivalence, for all values that 
+an Expression can have.
  *)
-
-Inductive RPN' : Set :=
-  | RPNlit' : lit -> RPN'
-  | RPNvar' : string -> RPN'
-  | RPNbinop' : RPN' -> RPN' -> (lit -> lit -> lit) -> RPN'
-.
-
-Fixpoint rpn' (e:Exp) {struct e} : RPN' :=
-match e with
-| Elit l => RPNlit' l
-| Evar x => RPNvar' x
-| Eplus e1 e2 => RPNbinop' (rpn' e1) (rpn' e2) plus
-| Emin  e1 e2 => RPNbinop' (rpn' e1) (rpn' e2) min
-| Emult e1 e2 => RPNbinop' (rpn' e1) (rpn' e2) mult
-end.
-
-Inductive exprpn_rel : Exp -> RPN' -> Prop :=
-    RPNl : forall n:lit     , exprpn_rel (Elit n) (RPNlit' n)
-  | RPNv : forall v:string  , exprpn_rel (Evar v) (RPNvar' v)
-  | RPNb0 : forall e1 e2:Exp, exprpn_rel (Eplus e1 e2) (RPNbinop' (rpn' e1) (rpn' e2) plus)
-  | RPNb1 : forall e1 e2:Exp, exprpn_rel (Emin  e1 e2) (RPNbinop' (rpn' e1) (rpn' e2) min)
-  | RPNb2 : forall e1 e2:Exp, exprpn_rel (Emult e1 e2) (RPNbinop' (rpn' e1) (rpn' e2) mult)
-.
-
-Lemma AllExpRelateToTheSameRPN : forall e:Exp, exprpn_rel e (rpn' e).
-Proof.
-  induction e; simpl.
-  - apply RPNl.
-  - apply RPNv.
-  - apply RPNb0.
-  - apply RPNb1.
-  - apply RPNb2.
-Qed.
-
